refactor: Some refactors of intro example

examples/scalaEquivalenceBenchmarkExamples/incomplete/intro.dfy
@@ -3,7 +3,7 @@
 datatype List<T> = Nil | Cons(head: T, tail: List<T>)
 
 function insertM(xs: List<int>, t: int): List<int>
-  {
+  decreases xs {
   match xs {
     case Nil => Cons(t, Nil)
     case Cons(hd, tl) =>
@@ -12,46 +12,43 @@ function insertM(xs: List<int>, t: int): List<int>
   }
 }
 
-function loopM<Seed>(seed: Seed, next: Seed -> (Seed, int), count: int, xs: List<int>): List<int>
-  decreases count {
+function insertRandomSortedM<Seed>(seed: Seed, next: Seed -> (Seed, int), count: int, xs: List<int>): List<int>
+  {
   if (count <= 0) then xs
   else
     var (nxtS, t) := next(seed);
-    loopM(nxtS, next, count - 1, insertM(xs, t))
+    insertRandomSortedM(nxtS, next, count - 1, insertM(xs, t))
 }
 
-function insertSorted5(t: int, xs: List<int>): List<int>
-  {
+function insert1(t: int, xs: List<int>): List<int>
+  decreases xs {
   match xs {
     case Nil => Cons(t, Nil)
     case Cons(hd, tl) =>
       if (t <= hd) then Cons(t, xs)
-      else Cons(hd, insertSorted5(t, tl))
+      else Cons(hd, insert1(t, tl))
   }
 }
 
-function go5<Seed>(seed: Seed, next: Seed -> (Seed, int), xs: List<int>, count: int): List<int>
+function insertRandomSorted1<Seed>(seed: Seed, next: Seed -> (Seed, int), xs: List<int>, count: int): List<int>
   decreases count {
   if (count <= 0) then xs
   else
     var (nxtS, t) := next(seed);
-    go5(nxtS, next, insertSorted5(t, xs), count - 1)
+    insertRandomSorted1(nxtS, next, insert1(t, xs), count - 1)
 }
 
-lemma equivalenceInsertSorted5(t: int, xs: List<int>)
-  ensures (insertSorted5(t, xs) == insertM(xs, t))
+lemma equivalenceInsert(t: int, xs: List<int>)
+  ensures (insert1(t, xs) == insertM(xs, t))
 {}
 
-lemma equivalenceGo5<Seed>(seed: Seed,
-                             next: Seed -> (Seed, int),
-                             xs: List<int>,
-                             count: int)
-  ensures (go5(seed, next, xs, count) == loopM(seed, next, count, xs))
+lemma equivalenceInsertRandomSorted<Seed>(seed: Seed, next: Seed -> (Seed, int), xs: List<int>, count: int)
+  ensures (insertRandomSorted1(seed, next, xs, count) == insertRandomSortedM(seed, next, count, xs))
   decreases count
 {
   if count > 0 {
     var (nxtS, t) := next(seed);
-    equivalenceGo5(nxtS, next, insertSorted5(t, xs), count - 1);
-    equivalenceInsertSorted5(t, xs);
+    equivalenceInsertRandomSorted(nxtS, next, insert1(t, xs), count - 1);
+    equivalenceInsert(t, xs);
   }
 }
